Progress ODH

src/tls/ODH.fst
@@ -65,7 +65,9 @@ let extract k g role ks s n =
     HKDF.hkdf_extract k n ikm
 
 (**************************************************************************)
+(** A simple idealization of CommonDH that records honestly generated shares *)
 module DH
+module MS = MonotoneSet
 
 type group
 val strongGroup: g:group -> GTot bool
@@ -78,7 +80,7 @@ val share_exponent: #g:group -> s:share g{hasExp s} -> Tot (exponent g)
 private let dh_region:rgn = new_region tls_tables_region
 private type share_table =
   (if Flags.ideal_kef then
-    monotone_set dh_region (g:group & s:share g) grows
+    MS.t dh_region (g:group & s:share g) grows
   else
     ())
 
@@ -90,8 +92,15 @@ abstract let share_log: share_table =
 
 abstract type honest_share (#g:group) (s:share g) =
   (if Flags.ideal_kef then
-    witnessed (fun h -> MS.contains (MS.m_sel h share_log) (g,s))
-  else False)
+    witnessed (MS.contains share_log (g,s))
+  else True)
+
+let is_honest (#g:group) (s:share g) : ST bool
+  (requires (fun h0 -> True))
+  (ensures (fun h0 b h1 ->
+    modifies_none h0 h1 /\
+    b <==> honest_share s)) =
+  Some? (MS.lookup share_log (g,s))
 
 let keygen (g:group) : ST (s:share g{hasExp s})
   (requires (fun h0 -> True))
@@ -99,7 +108,7 @@ let keygen (g:group) : ST (s:share g{hasExp s})
     honest_share s /\
     if Flags.ideal_kef then
       modifies_one dh_region h0 h1 /\
-      MS.m_sel h1 share_log == Set.union (MS.m_sel h0 share_log) (Set.singleton (g, s))
+      MR.m_sel h1 share_log == Set.union (MR.m_sel h0 share_log) (Set.singleton (g, s))
     else
       h0 = h1
   ))
@@ -108,7 +117,7 @@ let keygen (g:group) : ST (s:share g{hasExp s})
   if Flags.ideal_kef then begin
     MR.m_recall share_log;
     MS.append share_log (g,share);
-    witness (MS.contains (MS.m_read share_log) (g,share))
+    witness share_log (MS.contains share_log (g,share))
   end;
   share
 
@@ -144,12 +153,17 @@ type id = {
   kef_type: kef_type;
 }
 
-type role =
+type dhrole =
   | Initiator
   | Responder
 
+type role (i:id) =
+  (match i.kef_type with
+  | DH _ _ _ | DH_PSK _ _ _ _ -> dhrole
+  | _ -> unit)
+
 // The type of the input key material to extract
-type ikm (i:id) (ir:role) =
+type ikm (i:id) (ir:role i) =
   (match i.kef_type with
   | PSK pski -> PSK.psk pski
   | DH g si sr | DH_PSK _ g si sr ->
@@ -181,26 +195,38 @@ type extractor_instance (i:id) =
       KEF_PRF_ODH.state i)
 
 (* Global table of extractor instances indexed by id *)
-private let kef_region:rgn = new_region tls_tables_region
-private type kef_table =
+let kef_region:rgn = new_region tls_tables_region
+type kef_table =
   (if Flags.ideal_kef then
     MM.t kef_region id extractor_instance grows
   else
     ())
 
-abstract let kef_instances : kef_table =
+let kef_instances : kef_table =
   (if Flags.ideal_kef then
     MM.alloc #kef_region #id #extractor_instance #grows
   else
     ())
 
-let lookup_instance (i:id) =
+let lookup_instance (i:id) : ST (option (extractor_instance i))
+  (requires (fun h0 -> True))
+  (ensures (fun h0 sto h1 ->
+    modifies_none h0 h1 /\
+    if Flags.ideal_kef then
+      Some? sto ==> witnessed (MM.contains kef_instances i (Some?.v sto))
+    else
+      sto == None))
+  =
   if Flags.ideal_kef then
     MM.lookup kef_instances i
-  else None
+  else
+    None
 
-let extract_instance (#i:id) (st:extractor_instance i) (ir:role) (ikm:ikm i ir) (salt:salt i)
-  : ST (extracted_secret i)
+let extract_instance (#i:id) (st:extractor_instance i)
+  (ir:role) (ikm:ikm i ir) (salt:salt i) : ST (extracted_secret i)
+  (requires (fun h0 -> True))
+  (ensures (fun h0 r h1 ->
+    modifies_none h0 h1))
   =
   (match i.kef_type with
   | PSK _ | ZERO _ -> KEF_PRF.extract i st ir ikm salt
@@ -211,15 +237,19 @@ let extract_instance (#i:id) (st:extractor_instance i) (ir:role) (ikm:ikm i ir) 
     else
       KEF_PRF_ODH.extract i st ir ikm salt)
 
-let extract (i:id) (ir:role) (ikm:ikm i ir) (salt:salt i)
+let extract (i:id) (ir:role i) (ikm:ikm i ir) (salt:salt i)
   : ST (extracted_secret i)
   (requires (fun h0 -> True))
   (ensures (fun h0 s h1 -> h0=h1))
   =
-  match lookup_instance i with
-  | None ->
+  let st =
+    match lookup_instance i with
+    | Some st -> st
+    | None ->
+      (match i.kef_type with
+      | PSK pskid -> KEF_PRF.create
+        )
   | Some (st:extractor_instance i) =
-
 
 
 ///////////////////////////////////////////
@@ -227,27 +257,47 @@ let extract (i:id) (ir:role) (ikm:ikm i ir) (salt:salt i)
 module KEF_PRF
 open KEF
 
-type psk_id (i:id) =
-  is_PSK i.source \/ is_PSK_DHE i.source
-type id = i:id{psk_id i}
+type id = i:id{PSK? i.kef_type \/ ZERO? i.kef_type \/ DH_PSK? i.kef_type}
 
-let pskid (i:id) =
-  match i.source with
-  | PSK i -> i
-  | PSK_DHE i g -> i
+let safeId (i:id) =
+  (match i.kef_type with
+  | PSK pski -> PSK.safePSK pski
+  | ZERO hsId -> honest_hsId hsId
+  | DH_PSK esId _ _ _ -> honest_esId esId)
 
+(** Type of values used to key the PRF *)
+type prf_key (i:id) =
+  (match i.kef_type with
+  | PSK pski -> PSK.psk pski
+  | ZERO hsId -> expanded_secret (HandshakeSecretID hsId)
+  | DH_PSK esId _ _ _ -> expanded_secret (EarlySecretID esId))
+
+let prf_keylen (i:id) =
+  (match i.kef_type with
+  | PSK pski -> PSK.psklen pski
+  | ZERO hsId -> hashlen (hsId_hash hsId)
+  | DH_PSK esId _ _ _ -> hashlen (esId_hash esId)
+
+(** Type of the domain of the keyed PRF *)
+type prf_domain (i:id) =
+  (match i.kef_type with
+  | PSK _ -> unit
+  | ZERO _ -> unit
+  | DH_PSK _ _ _ _ -> bytes
+
+type prf_range (i:id) (d:domain i) = extracted_secret i
+
+(* Compact style: only allocate log for idealized instances *)
 type log (i:id) (r:rgn) =
   (if Flags.ideal_kef /\ safeId i then
-    monotone_map #r bytes (extracted_secret i)
+    MM.t r (prf_domain i) (prf_range i)
   else
     unit)
-
-type key (i:id) = PSK.kexlen (pskid i)
 
 type state (i:id) =
   | State:
      r:rgn ->
-     key: key i
+     key: prf_key i
      log: log i r ->
      state i
 
@@ -257,62 +307,69 @@ let create (i:id) (parent:rgn) : ST (state i)
     modifies_none h0 h1 /\
     extends st.r parent /\
     stronger_fresh_region st.r h0 h1 /\
-    MM.m_sel h1 st.log == MM.empty_map))
+    if Flags.ideal_kef then
+      h1 `contains` st.log /\
+      MM.m_sel h1 st.log == MM.empty_map
+    else
+      True))
   =
   let r = new_region parent in
-  let key = Random.bytes (PSK.kexlen (pskid i)) in
+  let key : prf_key i = Bytes.random (prf_keylen i) in
   let log =
     if Flags.ideal_kef then
-      MM.alloc #r () // ...
+      MM.alloc #r #(prf_domain i) #(prf_range i) #grows
     else () in
   State r key log
 
-let coerce (i:id) (r:rgn) (k:key i) : ST (state i)
+let coerce (i:id) (r:rgn) (k:prf_key i) : ST (state i)
   (requires (fun h0 -> ~(safeId i)))
   (ensures (fun h0 st h1 -> h0 = h1))
   =
   State r k ()
 
-type fresh_input (i:id{safeId i}) (st:state i) (ikm:bytes) (h:mem) =
-  is_None (MM.sel (MR.m_sel h st.log) ikm)
-
-let compute (i:id) (st:state i) (ikm:bytes) : ST (extracted_secret i)
-  (requires (fun h0 -> safeId i ==> fresh_input i st ikm h0))
-  (ensures (fun h0 s h1 ->
-    if safeId i /\ Flags.ideal_kef then
-      modifies_one st.r h0 h1 /\
-      MM.m_sel h1 st.log == MM.upd (m_sel h0 st.log) ikm s) /\
-      witnessed (MM.contains (m_sel h1 st.log) ikm)
-    else h0 = h1
+let extract (i:id) (st:state i) (v:prf_domain i) : ST (prf_range i v)
+  (requires (fun h0 -> True))
+  (ensures (fun h0 r h1 ->
+    if Flags.ideal_kef /\ safeId i then
+      (match MM.sel (MR.m_sel h0 st.log) v with
+      | None ->
+        modifies_one st.r h0 h1 /\
+        MR.m_sel h1 st.log == MM.upd (MR.m_sel h0 st.log) v r) /\
+        witnessed (MM.contains st.log v r)
+      | Some r' ->
+        modifies_none h0 h1 /\
+        r' = r)
+    else
+      h0 = h1
   ))
   =
   if Flags.ideal_kef && safeId i then
-    let secret = Random.bytes (KEF.keflen i.alg) in
-    m_recall st.log;
-    MM.extend st.log ikm secret;
-    witness (is_Some (MM.lookup st.log ikm));
-    secret
+    (match MM.lookup st.log v with
+    | Some r -> r
+    | None ->
+      let r = Bytes.random (keflen i.alg) in
+      m_recall st.log;
+      MM.extend st.log v r; r)
   else
-    Hacl.KEF.compute (i.alg) ikm (st.key) // e.g. HKDF
+    let concrete_v =
+      (match i.kef_type with
+      | PSK pskid -> zH (PSK.pskid_hash pskid // TODO move from KeySchedule
+      | ZERO hsId -> zH (hsId_hash hsId)
+      | DH_PSK _ _ _ _ -> v) in
+    Hacl.KEF.extract (i.alg) st.key concrete_v // e.g. HKDF
 
 module KEF_PRF_ODH
 
-type odh_id (i:id) =
-  DH? i.kef_type \/ DH_PSK? i.kef_type
-type id = i:KEF.id{odh_id i}
+type id = i:KEF.id{DH? i.kef_type \/ DH_PSK? i.kef_type}
 
 let shares_of_id (i:id) =
   match i.kef_type with
   | DH g si sr -> (g, si, sr)
   | DH_PSK _ g si sr -> (g, si, sr)
 
-type ikm (i:id) (ir:role) =
-  (match i.kef_type with
-  | DH g si sr | DH_PSK _ g si sr ->
-    if ir = Initiator then
-      e:DH.exponent si{DH.hasExp si /\ DH.share_exponent si = e}
-    else
-      e:DH.exponent sr{DH.hasExp sr /\ DH.share_exponent sr = e})
+inline_for_extraction let safeId (i:id) : Tot bool =
+  let (g, si, sr) = shares_of_id i in
+  Flags.ideal_kef && DH.strongGroup g && DH.honest_share si && DH.honest_share sr
 
 type salt (i:id) =
   (match i.kef_type with
@@ -321,41 +378,78 @@ type salt (i:id) =
   | DH_PSK esId _ _ _ ->
     expanded_secret (EarlySecretID esId))
 
+type odh_extracted (i:id) (s:salt i) = extracted_secret i
+
+(* Type of g^xy DH secrets *)
+abstract type odh_key (i:id) =
+  let (g, _, _) = shares_of_id i in
+  b:mlbytes (CommonDH.sharelen g)
+
+type log (i:id) (r:rgn) =
+  (if safeId i then
+    MM.t r (salt i) (odh_extracted i)
+  else
+    unit)
+
 type state (i:id) =
-  | State: log: monotone_map (i:id & l:label i) (extracted_secret) -> state i
+  | State:
+    r: rgn ->
+    key: odh_key i ->
+    log: log i r ->
+    state i
 
-let extract (i:id) (st:state i) (ir:role) (ikm:ikm i ir) (s:salt i)
-  : ST (extracted_secret i)
+let create (i:id) (ir:role i) (ikm:ikm i ir) : ST (state i)
   (requires (fun h0 -> True))
-  (ensures (fun h0 s h1 -> h0 = h1))
+  (ensures (fun h0 st h1 -> True))
   =
+  let r = new_region parent in
   let (g, si, sr) = shares_of_id i in
-  if Flags.ideal_kef && DH.is_honest si && DH.is_honest sr then
+  let honest = CommonDH.safeGroup g && CommonDH.is_honest si && CommonDH.is_honest sr in
+  let log =
+    if Flags.ideal_kef && honest then
+      MM.alloc #r #(salt i) #(odh_extracted i) #grows
+    else () in
+  let key = match ir with
+  | Initiator ->
+    let si_secret : (s:DH.share h{DH.hasExp s}) = fst ikm in
+    key = CommonDH.initiator g sr si_secret
+  | Responder ->
+    let si_secret : (s:DH.share h{DH.hasExp s}) = fst ikm in
+    let key = CommonDH.initiator g sr si_secret in
+    CommonDH.responder g si sr_secret in
+  State r key log
 
-  else
-    let ikm =
-      if ir = Initiator then
-        DH.exponentiate sr ikm
-      else
-        DH.exponentiate si ikm in
-    let s = Hacl.KEF.extract i.kefalg in
-    s
-
-let extract_responder k g s n =
-  let ks = keysharegen g in
-  if safeExtract k g ks s n then
-    (match m_lookup odh_table (k,g,s,pubshare ks,n) with
-    | None ->
-       let r = KDF.gen k in
-       update_map odh_table (k,g,s,pubshare ks,n) r; r
-    | Some r -> r)
-  else
-    let ikm = CommonDH.exponentiate g ks s in
-    ks, HKDF.hkdf_extract k n ikm
-
-let extract_initiator k g ks s n =
-    (match m_lookup odh_table (k,g, pubshare ks, s,n) with
+let extract (i:id) (st:state i) (ir:role i) (s:salt i)
+  : ST (odh_extracted i s)
+  (requires (fun h0 -> True))
+  (ensures (fun h0 r h1 ->
+    if Flags.ideal_kef /\ safeId i then
+      (match MM.sel (MR.m_sel h0 st.log) s with
+      | None ->
+        (ir == Initiator ==> modifies_none h0 h1) /\
+        (ir == Responder ==>
+          modifies_one st.r h0 h1 /\
+          MR.m_sel h1 st.log == MM.upd (MR.m_sel h0 st.log) s r /\
+          witnessed (MM.contains st.log s r))
+      | Some r' ->
+        modifies_none h0 h1 /\
+        r' = r)
+    else
+      h0 = h1))
+  =
+  let concrete_s =
+    match i.kef_type with
+    | DH _ _ _ -> zH (hashalg i)
+    | DH_PSK _ _ _ _ -> s in
+  let r = Hacl.KEF.extract (i.alg) st.key concrete_s in // e.g. HKDF
+  if Flags.ideal_kef && safeId i then
+    (match MM.lookup st.log v with
     | Some r -> r
     | None ->
-      let ikm = CommonDH.exponentiate g ks s in
-      HKDF.hkdf_extract k n ikm
+      if ir = Initiator then r
+      else begin
+        let r = Bytes.random (keflen i.alg) in
+        m_recall st.log;
+        MM.extend st.log v r; r
+      end)
+  else r
